Ticket13: more proof variants

src/tls/Benchmark.Ticket.fst
@@ -273,6 +273,523 @@ let write_ticket13_explicit_proof (tc: TC.ticketContents) (sl: LPB.slice) (pos: 
 
 (* here we are at 14 s, identifying the culprit for the framing lemmas (not the final modifies clause) *)
 
+let write_ticket13_explicit_proof_2 (tc: TC.ticketContents) (sl: LPB.slice) (pos: U32.t) : Stack U32.t
+  (requires (fun h -> LPB.live_slice h sl /\ U32.v pos <= U32.v sl.LPB.len /\ TC.T_ticket13? tc))
+  (ensures (fun h pos' h' ->
+    B.modifies (LPB.loc_slice_from sl pos) h h' /\ 
+    (
+    if pos' = LPB.max_uint32
+    then True
+    else
+      LPB.valid_content_pos TC.ticketContents_parser h' sl pos tc pos'
+  )))
+= let h0 = get () in
+  match tc with
+  | TC.T_ticket13 ({ TC13.cs=cs; TC13.rms=rms; TC13.nonce=nonce; TC13.creation_time=created; TC13.age_add=age; TC13.custom_data=custom }) ->
+    if (sl.LPB.len `U32.sub` pos) `U32.lt` (15ul `U32.add` len rms `U32.add` len nonce `U32.add` len custom)
+    then LPB.max_uint32
+    else begin
+//      assert (U32.v pos + 15 + U32.v (len rms) + U32.v (len nonce) + U32.v (len custom) <= U32.v sl.LPB.len);
+      let pos1 = pos `U32.add` 1ul in
+      let h1 = get () in
+      let pos2 = Parsers.CipherSuite.cipherSuite_writer cs sl pos1 in
+//      assert (U32.v pos2 <= U32.v pos1 + 2);
+      let h2 = get () in
+      let _ =
+        let l = LPB.loc_slice_from_to sl pos1 pos2 in
+        assume (B.loc_includes (LPB.loc_slice_from sl pos) l)
+      in
+      let len_rms = len rms in
+      let brms = B.sub sl.LPB.base (pos2 `U32.add` 1ul) len_rms in
+//      let _ = FStar.Bytes.store_bytes rms brms in
+      let _ = store_bytes rms brms in
+      let h31 = get () in
+      let _ =
+        let l = (B.loc_buffer brms) in
+        assume (B.loc_includes (LPB.loc_slice_from sl pos) l);
+        assume (B.loc_disjoint (LPB.loc_slice_from_to sl pos1 pos2) l);
+        LPB.valid_frame_strong Parsers.CipherSuite.cipherSuite_parser h2 sl pos1 l h31
+      in
+      let pos3 = Parsers.TicketContents13_rms.ticketContents13_rms_finalize sl pos2 len_rms in
+//      assert (U32.v pos3 <= U32.v pos2 + 1 + U32.v len_rms);
+      let h3 = get () in
+      let _ =
+        let l = LPB.loc_slice_from_to sl pos2 (pos2 `U32.add` 1ul) in
+        assume (B.loc_includes (LPB.loc_slice_from sl pos) l);
+        assume (B.loc_disjoint (LPB.loc_slice_from_to sl pos1 pos2) l);
+        LPB.valid_frame_strong Parsers.CipherSuite.cipherSuite_parser h31 sl pos1 l h3
+      in
+      let len_nonce = len nonce in
+      let bnonce = B.sub sl.LPB.base (pos3 `U32.add` 1ul) len_nonce in
+      let _ = store_bytes' nonce bnonce in
+//      let _ = if len_nonce <> 0ul then FStar.Bytes.store_bytes nonce bnonce in
+      let h41 = get () in
+      let _ =
+//        let l = if len_nonce <> 0ul then B.loc_buffer bnonce else B.loc_none in
+        let l = B.loc_buffer bnonce in
+        assume (B.loc_includes (LPB.loc_slice_from sl pos) l);
+        assume (B.loc_disjoint (LPB.loc_slice_from_to sl pos1 pos2) l);
+        LPB.valid_frame_strong Parsers.CipherSuite.cipherSuite_parser h3 sl pos1 l h41;
+        assume (B.loc_disjoint (LPB.loc_slice_from_to sl pos2 pos3) l);
+        LPB.valid_frame_strong TC13.ticketContents13_rms_parser h3 sl pos2 l h41
+      in
+      let pos4 = Parsers.TicketContents13_nonce.ticketContents13_nonce_finalize sl pos3 len_nonce in
+//      assert (U32.v pos4 <= U32.v pos3 + 1 + U32.v len_nonce);
+      let h4 = get () in
+      let _ =
+        let l = LPB.loc_slice_from_to sl pos3 (pos3 `U32.add` 1ul) in
+        assume (B.loc_includes (LPB.loc_slice_from sl pos) l);
+        assume (B.loc_disjoint (LPB.loc_slice_from_to sl pos1 pos2) l);
+        LPB.valid_frame_strong Parsers.CipherSuite.cipherSuite_parser h41 sl pos1 l h4;
+        assume (B.loc_disjoint (LPB.loc_slice_from_to sl pos2 pos3) l);
+        LPB.valid_frame_strong TC13.ticketContents13_rms_parser h41 sl pos2 l h4
+      in
+      let pos5 = LPI.write_u32 created sl pos4 in
+//      assert (U32.v pos5 <= U32.v pos4 + 4);
+      let h5 = get () in
+      let _ =
+        let l = LPB.loc_slice_from_to sl pos4 pos5 in
+        assume (B.loc_includes (LPB.loc_slice_from sl pos) l);
+        assume (B.loc_disjoint (LPB.loc_slice_from_to sl pos1 pos2) l);
+        LPB.valid_frame_strong Parsers.CipherSuite.cipherSuite_parser h4 sl pos1 l h5;
+        assume (B.loc_disjoint (LPB.loc_slice_from_to sl pos2 pos3) l);
+        LPB.valid_frame_strong TC13.ticketContents13_rms_parser h4 sl pos2 l h5;
+        assume (B.loc_disjoint (LPB.loc_slice_from_to sl pos3 pos4) l);
+        LPB.valid_frame_strong TC13.ticketContents13_nonce_parser h4 sl pos3 l h5
+      in
+      let pos6 = LPI.write_u32 age sl pos5 in
+//      assert (U32.v pos6 <= U32.v pos5 + 4);
+      let h6 = get () in
+      let _ =
+        let l = LPB.loc_slice_from_to sl pos5 pos6 in
+        assume (B.loc_includes (LPB.loc_slice_from sl pos) l);
+        assume (B.loc_disjoint (LPB.loc_slice_from_to sl pos1 pos2) l);
+        LPB.valid_frame_strong Parsers.CipherSuite.cipherSuite_parser h5 sl pos1 l h6;
+        assume (B.loc_disjoint (LPB.loc_slice_from_to sl pos2 pos3) l);
+        LPB.valid_frame_strong TC13.ticketContents13_rms_parser h5 sl pos2 l h6;
+        assume (B.loc_disjoint (LPB.loc_slice_from_to sl pos3 pos4) l);
+        LPB.valid_frame_strong TC13.ticketContents13_nonce_parser h5 sl pos3 l h6;
+        assume (B.loc_disjoint (LPB.loc_slice_from_to sl pos4 pos5) l);
+        LPB.valid_frame_strong LPI.parse_u32 h5 sl pos4 l h6
+      in
+      let len_custom = len custom in
+      let bcustom = B.sub sl.LPB.base (pos6 `U32.add` 2ul) len_custom in
+//      let _ = if len_custom <> 0ul then FStar.Bytes.store_bytes custom bcustom in
+      let _ = store_bytes' custom bcustom in
+      let h71 = get () in
+        let _ =
+//        let l = if len_custom <> 0ul then B.loc_buffer bcustom else B.loc_none in
+        let l = B.loc_buffer bcustom in
+        assume (B.loc_includes (LPB.loc_slice_from sl pos) l);
+        assume (B.loc_disjoint (LPB.loc_slice_from_to sl pos1 pos2) l);
+        LPB.valid_frame_strong Parsers.CipherSuite.cipherSuite_parser h6 sl pos1 l h71;
+        assume (B.loc_disjoint (LPB.loc_slice_from_to sl pos2 pos3) l);
+        LPB.valid_frame_strong TC13.ticketContents13_rms_parser h6 sl pos2 l h71;
+        assume (B.loc_disjoint (LPB.loc_slice_from_to sl pos3 pos4) l);
+        LPB.valid_frame_strong TC13.ticketContents13_nonce_parser h6 sl pos3 l h71;
+        assume (B.loc_disjoint (LPB.loc_slice_from_to sl pos4 pos5) l);
+        LPB.valid_frame_strong LPI.parse_u32 h6 sl pos4 l h71;
+        assume (B.loc_disjoint (LPB.loc_slice_from_to sl pos5 pos6) l);
+        LPB.valid_frame_strong LPI.parse_u32 h6 sl pos5 l h71
+      in
+//      assert (U32.v pos6 + 2 <= U32.v sl.LPB.len);
+      let pos7 = Parsers.TicketContents13_custom_data.ticketContents13_custom_data_finalize sl pos6 len_custom in
+//      assert (U32.v pos7 <= U32.v pos6 + 2 + U32.v len_custom);
+      let h7 = get () in
+        let _ =
+        let l = LPB.loc_slice_from_to sl pos6 (pos6 `U32.add` 2ul) in
+        assume (B.loc_includes (LPB.loc_slice_from sl pos) l);
+        assume (B.loc_disjoint (LPB.loc_slice_from_to sl pos1 pos2) l);
+        LPB.valid_frame_strong Parsers.CipherSuite.cipherSuite_parser h71 sl pos1 l h7;
+        assume (B.loc_disjoint (LPB.loc_slice_from_to sl pos2 pos3) l);
+        LPB.valid_frame_strong TC13.ticketContents13_rms_parser h71 sl pos2 l h7;
+        assume (B.loc_disjoint (LPB.loc_slice_from_to sl pos3 pos4) l);
+        LPB.valid_frame_strong TC13.ticketContents13_nonce_parser h71 sl pos3 l h7;
+        assume (B.loc_disjoint (LPB.loc_slice_from_to sl pos4 pos5) l);
+        LPB.valid_frame_strong LPI.parse_u32 h71 sl pos4 l h7;
+        assume (B.loc_disjoint (LPB.loc_slice_from_to sl pos5 pos6) l);
+        LPB.valid_frame_strong LPI.parse_u32 h71 sl pos5 l h7
+      in
+      let h = get () in
+      Parsers.TicketContents13.ticketContents13_valid h sl (pos `U32.add` 1ul);
+      Parsers.TicketContents.finalize_ticketContents_ticket13 sl pos;
+      assume (B.loc_includes (LPB.loc_slice_from sl pos) (LPB.loc_slice_from_to sl pos (pos `U32.add` 1ul)));
+      pos7
+    end
+
+let write_ticket13_explicit_proof_3 (tc: TC.ticketContents) (sl: LPB.slice) (pos: U32.t) : Stack U32.t
+  (requires (fun h -> LPB.live_slice h sl /\ U32.v pos <= U32.v sl.LPB.len /\ TC.T_ticket13? tc))
+  (ensures (fun h pos' h' ->
+    B.modifies (LPB.loc_slice_from sl pos) h h' /\ 
+    (
+    if pos' = LPB.max_uint32
+    then True
+    else
+      LPB.valid_content_pos TC.ticketContents_parser h' sl pos tc pos'
+  )))
+= let h0 = get () in
+  match tc with
+  | TC.T_ticket13 ({ TC13.cs=cs; TC13.rms=rms; TC13.nonce=nonce; TC13.creation_time=created; TC13.age_add=age; TC13.custom_data=custom }) ->
+    if (sl.LPB.len `U32.sub` pos) `U32.lt` (15ul `U32.add` len rms `U32.add` len nonce `U32.add` len custom)
+    then LPB.max_uint32
+    else begin
+//      assert (U32.v pos + 15 + U32.v (len rms) + U32.v (len nonce) + U32.v (len custom) <= U32.v sl.LPB.len);
+      let pos1 = pos `U32.add` 1ul in
+      let h1 = get () in
+      let pos2 = Parsers.CipherSuite.cipherSuite_writer cs sl pos1 in
+//      assert (U32.v pos2 <= U32.v pos1 + 2);
+      let h2 = get () in
+      let _ =
+        let l = LPB.loc_slice_from_to sl pos1 pos2 in
+        LPB.loc_includes_loc_slice_from_loc_slice_from_to sl pos pos1 pos2
+      in
+      let len_rms = len rms in
+      let brms = B.sub sl.LPB.base (pos2 `U32.add` 1ul) len_rms in
+//      let _ = FStar.Bytes.store_bytes rms brms in
+      let _ = store_bytes rms brms in
+      let h31 = get () in
+      let _ =
+        let l = (B.loc_buffer brms) in
+        LPB.loc_slice_from_includes_gsub sl pos sl.LPB.base (pos2 `U32.add` 1ul) len_rms;
+        LPB.loc_slice_from_to_gsub_disjoint sl sl.LPB.base pos pos2 (pos2 `U32.add` 1ul) len_rms;
+        LPB.valid_frame_strong Parsers.CipherSuite.cipherSuite_parser h2 sl pos1 l h31
+      in
+      let pos3 = Parsers.TicketContents13_rms.ticketContents13_rms_finalize sl pos2 len_rms in
+//      assert (U32.v pos3 <= U32.v pos2 + 1 + U32.v len_rms);
+      let h3 = get () in
+      let _ =
+        let l = LPB.loc_slice_from_to sl pos2 (pos2 `U32.add` 1ul) in
+        LPB.loc_includes_loc_slice_from_loc_slice_from_to sl pos pos2 (pos2 `U32.add` 1ul);
+        LPB.loc_slice_from_to_disjoint sl pos1 pos2 pos2 (pos2 `U32.add` 1ul);
+        LPB.valid_frame_strong Parsers.CipherSuite.cipherSuite_parser h31 sl pos1 l h3
+      in
+      let len_nonce = len nonce in
+      let bnonce = B.sub sl.LPB.base (pos3 `U32.add` 1ul) len_nonce in
+      let _ = store_bytes' nonce bnonce in
+//      let _ = if len_nonce <> 0ul then FStar.Bytes.store_bytes nonce bnonce in
+      let h41 = get () in
+      let _ =
+//        let l = if len_nonce <> 0ul then B.loc_buffer bnonce else B.loc_none in
+        let l = B.loc_buffer bnonce in
+        LPB.loc_slice_from_includes_gsub sl pos sl.LPB.base (pos3 `U32.add` 1ul) len_nonce;
+        LPB.loc_slice_from_to_gsub_disjoint sl sl.LPB.base pos1 pos2 (pos3 `U32.add` 1ul) len_nonce;
+        LPB.valid_frame_strong Parsers.CipherSuite.cipherSuite_parser h3 sl pos1 l h41;
+        LPB.loc_slice_from_to_gsub_disjoint sl sl.LPB.base pos2 pos3 (pos3 `U32.add` 1ul) len_nonce;
+        LPB.valid_frame_strong TC13.ticketContents13_rms_parser h3 sl pos2 l h41
+      in
+      let pos4 = Parsers.TicketContents13_nonce.ticketContents13_nonce_finalize sl pos3 len_nonce in
+//      assert (U32.v pos4 <= U32.v pos3 + 1 + U32.v len_nonce);
+      let h4 = get () in
+      let _ =
+        let l = LPB.loc_slice_from_to sl pos3 (pos3 `U32.add` 1ul) in
+        LPB.loc_includes_loc_slice_from_loc_slice_from_to sl pos pos3 (pos3 `U32.add` 1ul);
+        LPB.loc_slice_from_to_disjoint sl pos1 pos2 pos3 (pos3 `U32.add` 1ul);
+        LPB.valid_frame_strong Parsers.CipherSuite.cipherSuite_parser h41 sl pos1 l h4;
+        LPB.loc_slice_from_to_disjoint sl pos2 pos3 pos3 (pos3 `U32.add` 1ul);
+        LPB.valid_frame_strong TC13.ticketContents13_rms_parser h41 sl pos2 l h4
+      in
+      let pos5 = LPI.write_u32 created sl pos4 in
+//      assert (U32.v pos5 <= U32.v pos4 + 4);
+      let h5 = get () in
+      let _ =
+        let l = LPB.loc_slice_from_to sl pos4 pos5 in
+        LPB.loc_includes_loc_slice_from_loc_slice_from_to sl pos pos4 pos5;
+        LPB.loc_slice_from_to_disjoint sl pos1 pos2 pos4 pos5;
+        LPB.valid_frame_strong Parsers.CipherSuite.cipherSuite_parser h4 sl pos1 l h5;
+        LPB.loc_slice_from_to_disjoint sl pos2 pos3 pos4 pos5;
+        LPB.valid_frame_strong TC13.ticketContents13_rms_parser h4 sl pos2 l h5;
+        LPB.loc_slice_from_to_disjoint sl pos3 pos4 pos4 pos5;
+        LPB.valid_frame_strong TC13.ticketContents13_nonce_parser h4 sl pos3 l h5
+      in
+      let pos6 = LPI.write_u32 age sl pos5 in
+//      assert (U32.v pos6 <= U32.v pos5 + 4);
+      let h6 = get () in
+      let _ =
+        let l = LPB.loc_slice_from_to sl pos5 pos6 in
+        LPB.loc_includes_loc_slice_from_loc_slice_from_to sl pos pos5 pos6;
+        LPB.loc_slice_from_to_disjoint sl pos1 pos2 pos5 pos6;
+        LPB.valid_frame_strong Parsers.CipherSuite.cipherSuite_parser h5 sl pos1 l h6;
+        LPB.loc_slice_from_to_disjoint sl pos2 pos3 pos5 pos6;
+        LPB.valid_frame_strong TC13.ticketContents13_rms_parser h5 sl pos2 l h6;
+        LPB.loc_slice_from_to_disjoint sl pos3 pos4 pos5 pos6;
+        LPB.valid_frame_strong TC13.ticketContents13_nonce_parser h5 sl pos3 l h6;
+        LPB.loc_slice_from_to_disjoint sl pos4 pos5 pos5 pos6;
+        LPB.valid_frame_strong LPI.parse_u32 h5 sl pos4 l h6
+      in
+      let len_custom = len custom in
+      let bcustom = B.sub sl.LPB.base (pos6 `U32.add` 2ul) len_custom in
+//      let _ = if len_custom <> 0ul then FStar.Bytes.store_bytes custom bcustom in
+      let _ = store_bytes' custom bcustom in
+      let h71 = get () in
+        let _ =
+//        let l = if len_custom <> 0ul then B.loc_buffer bcustom else B.loc_none in
+        let l = B.loc_buffer bcustom in
+        LPB.loc_slice_from_includes_gsub sl pos sl.LPB.base (pos6 `U32.add` 2ul) len_custom;
+        LPB.loc_slice_from_to_gsub_disjoint sl sl.LPB.base pos1 pos2 (pos6 `U32.add` 2ul) len_custom;
+        LPB.valid_frame_strong Parsers.CipherSuite.cipherSuite_parser h6 sl pos1 l h71;
+        LPB.loc_slice_from_to_gsub_disjoint sl sl.LPB.base pos2 pos3 (pos6 `U32.add` 2ul) len_custom;
+        LPB.valid_frame_strong TC13.ticketContents13_rms_parser h6 sl pos2 l h71;
+        LPB.loc_slice_from_to_gsub_disjoint sl sl.LPB.base pos3 pos4 (pos6 `U32.add` 2ul) len_custom;
+        LPB.valid_frame_strong TC13.ticketContents13_nonce_parser h6 sl pos3 l h71;
+        LPB.loc_slice_from_to_gsub_disjoint sl sl.LPB.base pos4 pos5 (pos6 `U32.add` 2ul) len_custom;
+        LPB.valid_frame_strong LPI.parse_u32 h6 sl pos4 l h71;
+        LPB.loc_slice_from_to_gsub_disjoint sl sl.LPB.base pos5 pos6 (pos6 `U32.add` 2ul) len_custom;
+        LPB.valid_frame_strong LPI.parse_u32 h6 sl pos5 l h71
+      in
+//      assert (U32.v pos6 + 2 <= U32.v sl.LPB.len);
+      let pos7 = Parsers.TicketContents13_custom_data.ticketContents13_custom_data_finalize sl pos6 len_custom in
+//      assert (U32.v pos7 <= U32.v pos6 + 2 + U32.v len_custom);
+      let h7 = get () in
+        let _ =
+        let l = LPB.loc_slice_from_to sl pos6 (pos6 `U32.add` 2ul) in
+        LPB.loc_includes_loc_slice_from_loc_slice_from_to sl pos pos6 (pos6 `U32.add` 2ul);
+        LPB.loc_slice_from_to_disjoint sl pos1 pos2 pos6 (pos6 `U32.add` 2ul);
+        LPB.valid_frame_strong Parsers.CipherSuite.cipherSuite_parser h71 sl pos1 l h7;
+        LPB.loc_slice_from_to_disjoint sl pos2 pos3 pos6 (pos6 `U32.add` 2ul);
+        LPB.valid_frame_strong TC13.ticketContents13_rms_parser h71 sl pos2 l h7;
+        LPB.loc_slice_from_to_disjoint sl pos3 pos4 pos6 (pos6 `U32.add` 2ul);
+        LPB.valid_frame_strong TC13.ticketContents13_nonce_parser h71 sl pos3 l h7;
+        LPB.loc_slice_from_to_disjoint sl pos4 pos5 pos6 (pos6 `U32.add` 2ul);
+        LPB.valid_frame_strong LPI.parse_u32 h71 sl pos4 l h7;
+        LPB.loc_slice_from_to_disjoint sl pos5 pos6 pos6 (pos6 `U32.add` 2ul);
+        LPB.valid_frame_strong LPI.parse_u32 h71 sl pos5 l h7
+      in
+      let h = get () in
+      Parsers.TicketContents13.ticketContents13_valid h sl (pos `U32.add` 1ul);
+      Parsers.TicketContents.finalize_ticketContents_ticket13 sl pos;
+      LPB.loc_includes_loc_slice_from_loc_slice_from_to sl pos pos (pos `U32.add` 1ul);
+      pos7
+    end
+
+let write_ticket13_explicit_proof_2_somewhat_implicit (tc: TC.ticketContents) (sl: LPB.slice) (pos: U32.t) : Stack U32.t
+  (requires (fun h -> LPB.live_slice h sl /\ U32.v pos <= U32.v sl.LPB.len /\ TC.T_ticket13? tc))
+  (ensures (fun h pos' h' ->
+    B.modifies (LPB.loc_slice_from sl pos) h h' /\ 
+    (
+    if pos' = LPB.max_uint32
+    then True
+    else
+      LPB.valid_content_pos TC.ticketContents_parser h' sl pos tc pos'
+  )))
+= let h0 = get () in
+  match tc with
+  | TC.T_ticket13 ({ TC13.cs=cs; TC13.rms=rms; TC13.nonce=nonce; TC13.creation_time=created; TC13.age_add=age; TC13.custom_data=custom }) ->
+    if (sl.LPB.len `U32.sub` pos) `U32.lt` (15ul `U32.add` len rms `U32.add` len nonce `U32.add` len custom)
+    then LPB.max_uint32
+    else begin
+//      assert (U32.v pos + 15 + U32.v (len rms) + U32.v (len nonce) + U32.v (len custom) <= U32.v sl.LPB.len);
+      let pos1 = pos `U32.add` 1ul in
+      let h1 = get () in
+      let pos2 = Parsers.CipherSuite.cipherSuite_writer cs sl pos1 in
+//      assert (U32.v pos2 <= U32.v pos1 + 2);
+      let h2 = get () in
+      let _ =
+        let l = LPB.loc_slice_from_to sl pos1 pos2 in
+        assume (B.loc_includes (LPB.loc_slice_from sl pos) l)
+      in
+      let len_rms = len rms in
+      let brms = B.sub sl.LPB.base (pos2 `U32.add` 1ul) len_rms in
+//      let _ = FStar.Bytes.store_bytes rms brms in
+      let _ = store_bytes rms brms in
+      let h31 = get () in
+      let _ =
+        let l = (B.loc_buffer brms) in
+        assume (B.loc_includes (LPB.loc_slice_from sl pos) l);
+        LPB.valid_frame_strong Parsers.CipherSuite.cipherSuite_parser h2 sl pos1 l h31
+      in
+      let pos3 = Parsers.TicketContents13_rms.ticketContents13_rms_finalize sl pos2 len_rms in
+//      assert (U32.v pos3 <= U32.v pos2 + 1 + U32.v len_rms);
+      let h3 = get () in
+      let _ =
+        let l = LPB.loc_slice_from_to sl pos2 (pos2 `U32.add` 1ul) in
+        assume (B.loc_includes (LPB.loc_slice_from sl pos) l);
+        LPB.valid_frame_strong Parsers.CipherSuite.cipherSuite_parser h31 sl pos1 l h3
+      in
+      let len_nonce = len nonce in
+      let bnonce = B.sub sl.LPB.base (pos3 `U32.add` 1ul) len_nonce in
+      let _ = store_bytes' nonce bnonce in
+//      let _ = if len_nonce <> 0ul then FStar.Bytes.store_bytes nonce bnonce in
+      let h41 = get () in
+      let _ =
+//        let l = if len_nonce <> 0ul then B.loc_buffer bnonce else B.loc_none in
+        let l = B.loc_buffer bnonce in
+        assume (B.loc_includes (LPB.loc_slice_from sl pos) l);
+        LPB.valid_frame_strong Parsers.CipherSuite.cipherSuite_parser h3 sl pos1 l h41;
+        LPB.valid_frame_strong TC13.ticketContents13_rms_parser h3 sl pos2 l h41
+      in
+      let pos4 = Parsers.TicketContents13_nonce.ticketContents13_nonce_finalize sl pos3 len_nonce in
+//      assert (U32.v pos4 <= U32.v pos3 + 1 + U32.v len_nonce);
+      let h4 = get () in
+      let _ =
+        let l = LPB.loc_slice_from_to sl pos3 (pos3 `U32.add` 1ul) in
+        assume (B.loc_includes (LPB.loc_slice_from sl pos) l);
+        LPB.valid_frame_strong Parsers.CipherSuite.cipherSuite_parser h41 sl pos1 l h4;
+        LPB.valid_frame_strong TC13.ticketContents13_rms_parser h41 sl pos2 l h4
+      in
+      let pos5 = LPI.write_u32 created sl pos4 in
+//      assert (U32.v pos5 <= U32.v pos4 + 4);
+      let h5 = get () in
+      let _ =
+        let l = LPB.loc_slice_from_to sl pos4 pos5 in
+        assume (B.loc_includes (LPB.loc_slice_from sl pos) l);
+        LPB.valid_frame_strong Parsers.CipherSuite.cipherSuite_parser h4 sl pos1 l h5;
+        LPB.valid_frame_strong TC13.ticketContents13_rms_parser h4 sl pos2 l h5;
+        LPB.valid_frame_strong TC13.ticketContents13_nonce_parser h4 sl pos3 l h5
+      in
+      let pos6 = LPI.write_u32 age sl pos5 in
+//      assert (U32.v pos6 <= U32.v pos5 + 4);
+      let h6 = get () in
+      let _ =
+        let l = LPB.loc_slice_from_to sl pos5 pos6 in
+        assume (B.loc_includes (LPB.loc_slice_from sl pos) l);
+        LPB.valid_frame_strong Parsers.CipherSuite.cipherSuite_parser h5 sl pos1 l h6;
+        LPB.valid_frame_strong TC13.ticketContents13_rms_parser h5 sl pos2 l h6;
+        LPB.valid_frame_strong TC13.ticketContents13_nonce_parser h5 sl pos3 l h6;
+        LPB.valid_frame_strong LPI.parse_u32 h5 sl pos4 l h6
+      in
+      let len_custom = len custom in
+      let bcustom = B.sub sl.LPB.base (pos6 `U32.add` 2ul) len_custom in
+//      let _ = if len_custom <> 0ul then FStar.Bytes.store_bytes custom bcustom in
+      let _ = store_bytes' custom bcustom in
+      let h71 = get () in
+        let _ =
+//        let l = if len_custom <> 0ul then B.loc_buffer bcustom else B.loc_none in
+        let l = B.loc_buffer bcustom in
+        assume (B.loc_includes (LPB.loc_slice_from sl pos) l);
+        LPB.valid_frame_strong Parsers.CipherSuite.cipherSuite_parser h6 sl pos1 l h71;
+        LPB.valid_frame_strong TC13.ticketContents13_rms_parser h6 sl pos2 l h71;
+        LPB.valid_frame_strong TC13.ticketContents13_nonce_parser h6 sl pos3 l h71;
+        LPB.valid_frame_strong LPI.parse_u32 h6 sl pos4 l h71;
+        LPB.valid_frame_strong LPI.parse_u32 h6 sl pos5 l h71
+      in
+//      assert (U32.v pos6 + 2 <= U32.v sl.LPB.len);
+      let pos7 = Parsers.TicketContents13_custom_data.ticketContents13_custom_data_finalize sl pos6 len_custom in
+//      assert (U32.v pos7 <= U32.v pos6 + 2 + U32.v len_custom);
+      let h7 = get () in
+        let _ =
+        let l = LPB.loc_slice_from_to sl pos6 (pos6 `U32.add` 2ul) in
+        assume (B.loc_includes (LPB.loc_slice_from sl pos) l);
+        LPB.valid_frame_strong Parsers.CipherSuite.cipherSuite_parser h71 sl pos1 l h7;
+        LPB.valid_frame_strong TC13.ticketContents13_rms_parser h71 sl pos2 l h7;
+        LPB.valid_frame_strong TC13.ticketContents13_nonce_parser h71 sl pos3 l h7;
+        LPB.valid_frame_strong LPI.parse_u32 h71 sl pos4 l h7;
+        LPB.valid_frame_strong LPI.parse_u32 h71 sl pos5 l h7
+      in
+      let h = get () in
+      Parsers.TicketContents13.ticketContents13_valid h sl (pos `U32.add` 1ul);
+      Parsers.TicketContents.finalize_ticketContents_ticket13 sl pos;
+      assume (B.loc_includes (LPB.loc_slice_from sl pos) (LPB.loc_slice_from_to sl pos (pos `U32.add` 1ul)));
+      pos7
+    end
+
+let write_ticket13_explicit_proof_2_somewhat_implicit_2 (tc: TC.ticketContents) (sl: LPB.slice) (pos: U32.t) : Stack U32.t
+  (requires (fun h -> LPB.live_slice h sl /\ U32.v pos <= U32.v sl.LPB.len /\ TC.T_ticket13? tc))
+  (ensures (fun h pos' h' ->
+    B.modifies (LPB.loc_slice_from sl pos) h h' /\ 
+    (
+    if pos' = LPB.max_uint32
+    then True
+    else
+      LPB.valid_content_pos TC.ticketContents_parser h' sl pos tc pos'
+  )))
+= let h0 = get () in
+  match tc with
+  | TC.T_ticket13 ({ TC13.cs=cs; TC13.rms=rms; TC13.nonce=nonce; TC13.creation_time=created; TC13.age_add=age; TC13.custom_data=custom }) ->
+    if (sl.LPB.len `U32.sub` pos) `U32.lt` (15ul `U32.add` len rms `U32.add` len nonce `U32.add` len custom)
+    then LPB.max_uint32
+    else begin
+//      assert (U32.v pos + 15 + U32.v (len rms) + U32.v (len nonce) + U32.v (len custom) <= U32.v sl.LPB.len);
+      let pos1 = pos `U32.add` 1ul in
+      let h1 = get () in
+      let pos2 = Parsers.CipherSuite.cipherSuite_writer cs sl pos1 in
+//      assert (U32.v pos2 <= U32.v pos1 + 2);
+      let h2 = get () in
+      let len_rms = len rms in
+      let brms = B.sub sl.LPB.base (pos2 `U32.add` 1ul) len_rms in
+//      let _ = FStar.Bytes.store_bytes rms brms in
+      let _ = store_bytes rms brms in
+      let h31 = get () in
+      let _ =
+        let l = (B.loc_buffer brms) in
+        LPB.valid_frame_strong Parsers.CipherSuite.cipherSuite_parser h2 sl pos1 l h31
+      in
+      let pos3 = Parsers.TicketContents13_rms.ticketContents13_rms_finalize sl pos2 len_rms in
+//      assert (U32.v pos3 <= U32.v pos2 + 1 + U32.v len_rms);
+      let h3 = get () in
+      let _ =
+        let l = LPB.loc_slice_from_to sl pos2 (pos2 `U32.add` 1ul) in
+        LPB.valid_frame_strong Parsers.CipherSuite.cipherSuite_parser h31 sl pos1 l h3
+      in
+      let len_nonce = len nonce in
+      let bnonce = B.sub sl.LPB.base (pos3 `U32.add` 1ul) len_nonce in
+      let _ = store_bytes' nonce bnonce in
+//      let _ = if len_nonce <> 0ul then FStar.Bytes.store_bytes nonce bnonce in
+      let h41 = get () in
+      let _ =
+//        let l = if len_nonce <> 0ul then B.loc_buffer bnonce else B.loc_none in
+        let l = B.loc_buffer bnonce in
+        LPB.valid_frame_strong Parsers.CipherSuite.cipherSuite_parser h3 sl pos1 l h41;
+        LPB.valid_frame_strong TC13.ticketContents13_rms_parser h3 sl pos2 l h41
+      in
+      let pos4 = Parsers.TicketContents13_nonce.ticketContents13_nonce_finalize sl pos3 len_nonce in
+//      assert (U32.v pos4 <= U32.v pos3 + 1 + U32.v len_nonce);
+      let h4 = get () in
+      let _ =
+        let l = LPB.loc_slice_from_to sl pos3 (pos3 `U32.add` 1ul) in
+        LPB.valid_frame_strong Parsers.CipherSuite.cipherSuite_parser h41 sl pos1 l h4;
+        LPB.valid_frame_strong TC13.ticketContents13_rms_parser h41 sl pos2 l h4
+      in
+      let pos5 = LPI.write_u32 created sl pos4 in
+//      assert (U32.v pos5 <= U32.v pos4 + 4);
+      let h5 = get () in
+      let _ =
+        let l = LPB.loc_slice_from_to sl pos4 pos5 in
+        LPB.valid_frame_strong Parsers.CipherSuite.cipherSuite_parser h4 sl pos1 l h5;
+        LPB.valid_frame_strong TC13.ticketContents13_rms_parser h4 sl pos2 l h5;
+        LPB.valid_frame_strong TC13.ticketContents13_nonce_parser h4 sl pos3 l h5
+      in
+      let pos6 = LPI.write_u32 age sl pos5 in
+//      assert (U32.v pos6 <= U32.v pos5 + 4);
+      let h6 = get () in
+      let _ =
+        let l = LPB.loc_slice_from_to sl pos5 pos6 in
+        LPB.valid_frame_strong Parsers.CipherSuite.cipherSuite_parser h5 sl pos1 l h6;
+        LPB.valid_frame_strong TC13.ticketContents13_rms_parser h5 sl pos2 l h6;
+        LPB.valid_frame_strong TC13.ticketContents13_nonce_parser h5 sl pos3 l h6;
+        LPB.valid_frame_strong LPI.parse_u32 h5 sl pos4 l h6
+      in
+      let len_custom = len custom in
+      let bcustom = B.sub sl.LPB.base (pos6 `U32.add` 2ul) len_custom in
+//      let _ = if len_custom <> 0ul then FStar.Bytes.store_bytes custom bcustom in
+      let _ = store_bytes' custom bcustom in
+      let h71 = get () in
+        let _ =
+//        let l = if len_custom <> 0ul then B.loc_buffer bcustom else B.loc_none in
+        let l = B.loc_buffer bcustom in
+        LPB.valid_frame_strong Parsers.CipherSuite.cipherSuite_parser h6 sl pos1 l h71;
+        LPB.valid_frame_strong TC13.ticketContents13_rms_parser h6 sl pos2 l h71;
+        LPB.valid_frame_strong TC13.ticketContents13_nonce_parser h6 sl pos3 l h71;
+        LPB.valid_frame_strong LPI.parse_u32 h6 sl pos4 l h71;
+        LPB.valid_frame_strong LPI.parse_u32 h6 sl pos5 l h71
+      in
+//      assert (U32.v pos6 + 2 <= U32.v sl.LPB.len);
+      let pos7 = Parsers.TicketContents13_custom_data.ticketContents13_custom_data_finalize sl pos6 len_custom in
+//      assert (U32.v pos7 <= U32.v pos6 + 2 + U32.v len_custom);
+      let h7 = get () in
+        let _ =
+        let l = LPB.loc_slice_from_to sl pos6 (pos6 `U32.add` 2ul) in
+        LPB.valid_frame_strong Parsers.CipherSuite.cipherSuite_parser h71 sl pos1 l h7;
+        LPB.valid_frame_strong TC13.ticketContents13_rms_parser h71 sl pos2 l h7;
+        LPB.valid_frame_strong TC13.ticketContents13_nonce_parser h71 sl pos3 l h7;
+        LPB.valid_frame_strong LPI.parse_u32 h71 sl pos4 l h7;
+        LPB.valid_frame_strong LPI.parse_u32 h71 sl pos5 l h7
+      in
+      let h = get () in
+      Parsers.TicketContents13.ticketContents13_valid h sl (pos `U32.add` 1ul);
+      Parsers.TicketContents.finalize_ticketContents_ticket13 sl pos;
+      pos7
+    end
+
 #reset-options
 
 let write_ticket (tc: TC.ticketContents) (sl: LPB.slice) (pos: U32.t) : Stack U32.t
